Picinae_lifter_lifter.v
@@ -1,0 +1,455 @@
+Require Import Picinae_metarocq_prelude.
+Require Import NArith.
+Open Scope N.
+
+Compute $quote 5.
+(*
+Load MetaRocqPrelude.
+Import MonadNotation.
+From MetaRocq.Utils Require Import bytestring.
+Import String.
+Open Scope bs.
+ *)
+Parameter s : store.
+Parameter x:N.
+Parameter a:addr.
+
+
+Locate "<-".
+Require Import List.
+Print map.
+Print zxbits.
+
+Print tCase.
+Definition nat_id (n:nat) :=
+  match n with
+  | O => O
+  | S n' => n'
+  end.
+(* tCase : case_info -> predicate term -> term -> list (branch term) -> term
+    case_info: { ci_ind : inductive; ci_npar : nat; ci_relevance : relevance}
+      inductive: {inductive_mind: kername; inductive_ind: nat}
+      relevance: Relevant | Irrelevant
+    predicate: {puinst : Instance.t; pparams: list term; pcontext: list aname; preturn: term}
+      Instance.t: list Level.t (????)
+    branch: { bcontext: list aname; bbody: term }
+      aname: binder_annot name
+
+   Just map
+ *)
+Compute $quote(
+fun m P (PO : P 0) (PS : forall n, P (S n)) =>
+match m as n return P n with
+| 0 => PO
+| S n => PS n
+end
+)%nat.
+(*(
+tCase
+    {|
+      ci_ind :=
+        {|
+          inductive_mind :=
+            (MPfile ["Datatypes"; "Init"; "Corelib"], "nat");
+          inductive_ind := 0
+        |};
+      ci_npar := 0;
+      ci_relevance := Relevant
+    |}
+    {|
+      puinst := [];
+      pparams := [];
+      pcontext :=
+        [{|
+          binder_name := nNamed "n";
+          binder_relevance := Relevant
+        |}];
+      preturn := tApp (tRel 3) [tRel 0]
+    |} (tRel 3)
+    [{| bcontext := []; bbody := tRel 1 |};
+    {|
+      bcontext :=
+        [{|
+            binder_name := nNamed "n";
+            binder_relevance := Relevant
+          |}];
+      bbody := tApp (tRel 1) [tRel 0]
+      |}])
+*)
+Compute $quote nat.
+Notation "'_nat_'" := (tInd {| inductive_mind := (MPfile ["Datatypes"; "Init"; "Corelib"], "nat"); inductive_ind := 0 |} []).
+Notation "'_natind_'" := ({| inductive_mind := (MPfile ["Datatypes"; "Init"; "Corelib"], "nat"); inductive_ind := 0 |}).
+Compute $quote (fun n => match n with
+  | O => O
+  | S n' => O
+  end).
+(*= Lib.tLam "n" _nat_
+         (tCase
+            {| ci_ind := _natind_; ci_npar := 0; ci_relevance := Relevant |}
+            {|
+              puinst := [];
+              pparams := [];
+              pcontext :=
+                [{|
+                   binder_name := nNamed "n"; binder_relevance := Relevant
+                 |}];
+              preturn := _nat_
+            |} (tRel 0)
+            [{| bcontext := []; bbody := tConstruct _natind_ 0 [] |};
+             {|
+               bcontext :=
+                 [{|
+                    binder_name := nNamed "n'"; binder_relevance := Relevant
+                  |}];
+               bbody := tRel 0
+             |}])
+   : term*)
+Compute $quote_rec nat_id.
+
+Inductive color : Set :=
+  | Red (c:color): color
+  | Blue : color
+  | Dark (c:color) : color.
+
+Compute $quote color.
+Notation "'_color_'" := (tInd {| inductive_mind := (MPfile ["Picinae_lifter_lifter"; "Picinae"], "color"); inductive_ind := 0 |} []).
+Notation "'_colorind_'" := ({| inductive_mind := (MPfile ["Picinae_lifter_lifter"; "Picinae"], "color"); inductive_ind := 0 |}).
+(*MetaRocq Run (printQualid "color").*)
+Compute $quote (fun c => match c with
+                         | Dark c' => Dark c'
+                         | Red c' => Red c'
+                         | Blue => Blue
+                         end
+).
+
+Print List.
+About map.
+Print map.
+Fixpoint mapi_ {A B:Type} (f:nat->A->B) (n:nat) (l:list A) : list B :=
+  match l with
+  | [] => []
+  | h::t => f n h :: mapi_ f (Nat.succ n) t
+  end.
+Definition mapi {A B:Type} (f:nat->A->B) l := mapi_ f 0%nat l.
+
+MetaRocq Run (printQualid "color").
+
+Print mutual_inductive_body.
+Print tCase.
+Print name.
+Search inductive.
+Fixpoint tRel_desc (n:nat) :=
+  match n with
+  | O => [tRel O]
+  | S n'=> tRel n :: tRel_desc n'
+  end.
+Definition inductive_to_case (ind:inductive) : TemplateMonad term:=
+  mind <- tmQuoteInductive (inductive_mind ind);;
+  match nth_error (ind_bodies mind) (inductive_ind ind) with
+  | None => tmFail "inductive index out of bounds"
+  | Some indbody => let ctors := ind_ctors indbody in
+                    let branches := mapi (fun n c => match cstr_args c with
+                                                     | [] => {| bcontext := []; bbody := tConstruct ind n [] |}
+                                                     | _::_ => {| bcontext := map decl_name (cstr_args c); bbody := tApp (tConstruct ind n []) (tRel_desc (Nat.pred (length (cstr_args c))))|}
+                                                     end) ctors in
+                    tmReturn (tCase {| ci_ind := ind; ci_npar := 0; ci_relevance := Relevant |}
+                                    {| puinst := []; pparams := []; pcontext := [{| binder_name := nNamed "x"; binder_relevance := Relevant |}]; preturn := (tInd ind []) |}
+                                    (tRel 0%nat)
+                                    branches)
+  end.
+Definition qualid_identity (q:qualid) : TemplateMonad unit :=
+  glob_ref <- tmLocate1 q ;;
+  match glob_ref with
+  | IndRef ind => case <- inductive_to_case ind;; tmUnquote (tLambda {| binder_name := nNamed "x"; binder_relevance := Relevant |} (tInd ind []) case) >>= tmPrint
+  | _ => tmFail ("["++q++"] not a valid Inductive reference.")
+  end.
+
+MetaRocq Run (qualid_identity "term").
+
+(*= Lib.tLam "n" _nat_
+         (tCase
+            {| ci_ind := _natind_; ci_npar := 0; ci_relevance := Relevant |}
+            {|
+              puinst := [];
+              pparams := [];
+              pcontext :=
+                [{|
+                   binder_name := nNamed "n"; binder_relevance := Relevant
+                 |}];
+              preturn := _nat_
+            |} (tRel 0)
+            [{| bcontext := []; bbody := tConstruct _natind_ 0 [] |};
+             {|
+               bcontext :=
+                 [{|
+                    binder_name := nNamed "n'"; binder_relevance := Relevant
+                  |}];
+               bbody := tRel 0
+             |}])
+   : term*)
+
+
+Definition constructor_to_branch (tconstr:term) (cb:constructor_body) : branch term :=
+  match cstr_args cb with
+  | nil =>
+  let len := length (cstr_args cb) in
+  let bctxt := map decl_name (cstr_args cb) in
+  let bbdy := tApp (tConstruct )
+
+       ind_ctors :=
+         [{|
+            cstr_name := "Red";
+            cstr_args :=
+              [{|
+                 decl_name :=
+                   {|
+                     binder_name := nNamed "c"; binder_relevance := Relevant
+                   |};
+                 decl_body := None;
+                 decl_type := tRel 0
+               |}];
+            cstr_indices := [];
+            cstr_type := tPro "c" (tRel 0) (tRel 1);
+            cstr_arity := 1
+          |};
+          {|
+            cstr_name := "Blue";
+            cstr_args := [];
+            cstr_indices := [];
+            cstr_type := tRel 0;
+            cstr_arity := 0
+          |};
+          {|
+            cstr_name := "Dark";
+            cstr_args :=
+              [{|
+                 decl_name :=
+                   {|
+                     binder_name := nNamed "c"; binder_relevance := Relevant
+                   |};
+                 decl_body := None;
+                 decl_type := tRel 0
+               |}];
+            cstr_indices := [];
+            cstr_type := tPro "c" (tRel 0) (tRel 1);
+            cstr_arity := 1
+          |}];
+
+            [{|
+               bcontext :=
+                 [{|
+                    binder_name := nNamed "c'"; binder_relevance := Relevant
+                  |}];
+               bbody := tApp (tConstruct _colorind_ 0 []) [tRel 0]
+             |}; {| bcontext := []; bbody := tConstruct _colorind_ 1 [] |};
+             {|
+               bcontext :=
+                 [{|
+                    binder_name := nNamed "c'"; binder_relevance := Relevant
+                  |}];
+               bbody := tApp (tConstruct _colorind_ 2 []) [tRel 0]
+             |}])
+
+Definition printQualid (q : qualid): TemplateMonad unit :=
+  kn <- tmLocate1 q ;;
+  match kn with
+  | IndRef ind => tmPrint "Quoted inductive: ";; (*tmPrint ind;;*) mib <- (tmQuoteInductive ind.(inductive_mind));; (*tmPrint mib;;*)
+    match (ind_bodies mib) with
+    | h::nil => let casebody := ind_ctors h in tmPrint casebody
+    | _ => tmFail "Could not make identity for mutual inductive type."
+    end
+  | ConstRef kn => tmPrint "Quoted constant: ";; tmPrint kn;; (tmQuoteConstant kn false) >>= tmPrint
+  | _ => tmFail ("[" ++ q ++ "] is not an inductive")
+  end.
+
+MetaRocq Run (printQualid "nat").
+
+Fixpoint monadmap {A B:Type} (f:A->TemplateMonad B) (l:list A) : TemplateMonad (list B) :=
+  match l with
+  | h::t => fh <- f h;; ft <- monadmap f t;; tmReturn (fh::ft)
+  | nil => tmReturn nil
+  end.
+
+Time Definition Nify_fn (Nify:term -> TemplateMonad term) (fn:term) (ts:list term): TemplateMonad term :=
+  Nts <- monadmap Nify ts ;;
+  if fn == _zxbits_ then tmReturn (tApp _xbits_ Nts) else
+  if fn == _Z.of_N_ then (match ts with h::nil => Nify h | _ => tmFail "Z.of_N had more than one argument." end) else
+  if fn == _Z.eqb_ then tmReturn (tApp _N.eqb_ Nts) else
+  match fn with
+  | tConst kn _ => _fn_ <- tmQuoteConstant kn true ;;
+  tmReturn (tApp fn Nts).
+
+Notation "'_Npow_'" := (tConst (MPdot (MPfile ["BinNatDef"; "NArith"; "Stdlib"]) "N", "pow") []).
+
+Time Definition Nify_fn' (Nify:term -> TemplateMonad term) (fn:term) (ts:list term): TemplateMonad term :=
+  Nts <- monadmap Nify ts ;;
+  match fn with
+  | _Z.of_N_ => match ts with h::nil => Nify h | _ => tmFail "Z.of_N had more than one argument." end
+  | _Z.eqb_ => tmReturn (tApp _N.eqb_ Nts)
+  | _ => tmReturn (tApp fn Nts)
+  end.
+
+
+Compute $quote (if true then 1 else 2).
+Print tCase.
+Definition Nify_case (Nify:term -> TemplateMonad term)
+
+
+Fixpoint Nify t : TemplateMonad term :=
+  match t with
+  | tApp fn ts => Nify_fn Nify fn ts
+      (*| tApp _zxbits_ Zls => Nls <- monadmap Nify Zls ;; tmReturn (tApp _xbits_ Nls)
+    (*
+  | tApp _zxbits_ (Zx::Zlo::Zhi::nil) => Nx <- Nify Zx ;; Nlo <- Nify Zlo ;; Nhi <- Nify Zhi ;;
+      tmReturn (tApp _xbits_ (Nx::Nlo::Nhi::nil))
+      *)
+  | tApp _Z.of_N_ (n::nil) => tmReturn (Nify n)
+  | tApp _Z.eqb_ (Zl::Zr::nil) => tmReturn (tApp _N.eqb_ ((Nify Zl)::(Nify Zr)::nil))
+       *)
+  | _Z0_ => tmReturn (_0%N_)
+  | _Z1_ => tmReturn (_1%N_)
+  | _Z2_ => tmReturn (_2%N_)
+  | _Z3_ => tmReturn (_3%N_)
+  | _Z4_ => tmReturn (_4%N_)
+  | _Z5_ => tmReturn (_5%N_)
+  | _Z6_ => tmReturn (_6%N_)
+  | _Z7_ => tmReturn (_7%N_)
+  | _Z8_ => tmReturn (_8%N_)
+  | _Z9_ => tmReturn (_9%N_)
+  | _Z10_ => tmReturn (_10%N_)
+  | _Z11_ => tmReturn (_11%N_)
+  | _Z12_ => tmReturn (_12%N_)
+  | _Z13_ => tmReturn (_13%N_)
+  | _Z14_ => tmReturn (_14%N_)
+  | _Z15_ => tmReturn (_15%N_)
+  | _Z16_ => tmReturn (_16%N_)
+  | _Z17_ => tmReturn (_17%N_)
+  | _Z18_ => tmReturn (_18%N_)
+  | _Z19_ => tmReturn (_19%N_)
+  | _Z20_ => tmReturn (_20%N_)
+  | _Z21_ => tmReturn (_21%N_)
+  | _Z22_ => tmReturn (_22%N_)
+  | _Z23_ => tmReturn (_23%N_)
+  | _Z24_ => tmReturn (_24%N_)
+  | _Z25_ => tmReturn (_25%N_)
+  | _Z26_ => tmReturn (_26%N_)
+  | _Z27_ => tmReturn (_27%N_)
+  | _Z28_ => tmReturn (_28%N_)
+  | _Z29_ => tmReturn (_29%N_)
+  | _Z30_ => tmReturn (_30%N_)
+  | _Z31_ => tmReturn (_31%N_)
+  | _Z32_ => tmReturn (_32%N_)
+  | _Z4095_ => tmReturn (_4095%N_)
+  | _ => tmReturn (t)
+  end.
+Locate "=?".
+
+Compute ($quote (zxbits Z1 Z1 Z1)).
+Compute Nify ($quote (zxbits Z1 Z1 Z1)).
+
+Compute (is_positivequot ($quote 4%positive)).
+Check arm2il : addr -> arm_inst -> stmt.
+Check arm_decode : BinNums.Z -> arm_inst.
+
+(* Try to create an arm2il that eliminates intermediate uses of arm_inst everywhere.
+   That is a difficult datatype to reify into exp. *)
+Timeout 10 Eval hnf in arm2il a (arm_decode (Z.of_N x)).
+Eval unfold arm2il, arm_decode2il, arm_decode_64bit_transfer2il, arm_decode_8_16_32bit_transfer2il, arm_decode_b2il, arm_decode_bfx2il, arm_decode_bkpt2il, arm_decode_bl2il, arm_decode_blx_i2il, arm_decode_blx_r2il, arm_decode_branch_block_transfer2il, arm_decode_bx2il, arm_decode_bxj2il, arm_decode_clz2il, arm_decode_coprocessor2il, arm_decode_coproc_m2il, arm_decode_data_i2il, arm_decode_data_misc2il, arm_decode_data_processing2il, arm_decode_data_r2il, arm_decode_data_rd02il, arm_decode_data_rn02il, arm_decode_data_rsr2il, arm_decode_extend2il, arm_decode_extra_load_store2il, arm_decode_extra_ls_i2il, arm_decode_extra_ls_r2il, arm_decode_floating_data_processing2il, arm_decode_halfword_multiply2il, arm_decode_hint2il, arm_decode_hmul2il, arm_decode_load_store2il, arm_decode_ls_i2il,
+arm_decode_lsm2il, arm_decode_ls_r2il, arm_decode_media2il, arm_decode_mem_hint_simd2il, arm_decode_misc2il, arm_decode_mov_wt2il, arm_decode_msr_hints2il,
+arm_decode_mul2il, arm_decode_multiply2il, arm_decode_packing2il, arm_decode_parallel_add_sub2il, arm_decode_pas2il, arm_decode_pld_i2il, arm_decode_pld_r2il, arm_decode_rev2il, arm_decode_sat2il, arm_decode_saturating_add_sub2il,
+arm_decode_signed_multiply2il, arm_decode_simd2il, arm_decode_svc2il, arm_decode_sync_l2il, arm_decode_sync_primitives2il, arm_decode_sync_s2il, arm_decode_unconditional2il, arm_decode_vcmp2il, arm_decode_vcvt_ds2il, arm_decode_vcvt_fpf2il, arm_decode_vcvt_fpi2il, arm_decode_vfp2il,
+arm_decode_vfp_other2il, arm_decode_vls2il, arm_decode_vlsm2il, arm_decode_vmov_i2il, arm_decode_vmov_r12il, arm_decode_vmov_r22il, arm_decode_vmrs2il, arm_decode_vreg_ls2il,
+arm_decode_vls2il, arm_decode_64bit_transfer2il, arm_decode_8_16_32bit_transfer2il, arm_decode_b2il, arm_decode_bfx2il, arm_decode_bkpt2il, arm_decode_bl2il, arm_decode_blx_i2il, arm_decode_blx_r2il, arm_decode_bx2il, arm_decode_bxj2il, arm_decode_clz2il, arm_decode_data_i2il, arm_decode_extend2il, arm_decode_hint2il, arm_decode_mem_hint_simd2il, arm_decode_mul2il, arm_decode_sat2il, arm_decode_sync_l2il, arm_decode_vlsm2il,
+arm_decode_pld_i2il, arm_decode_pld_r2il, arm_decode_simd2il, arm_decode_vmov_r12il, arm_decode_vmov_r22il, arm_decode_vmrs2il
+in (arm_decode2il (Z.of_N x) (arm2il a)).
+Timeout 10 Eval simpl in (arm_decode2il (Z.of_N x) (arm2il a)).
+Goal forall z, z = arm_decode2il (Z.of_N x) (arm2il a).
+intros.
+unfold arm_decode2il.
+unfold arm_decode2il, arm_decode_64bit_transfer2il, arm_decode_8_16_32bit_transfer2il, arm_decode_b2il, arm_decode_bfx2il, arm_decode_bkpt2il, arm_decode_bl2il, arm_decode_blx_i2il, arm_decode_blx_r2il, arm_decode_branch_block_transfer2il, arm_decode_bx2il, arm_decode_bxj2il, arm_decode_clz2il, arm_decode_coprocessor2il, arm_decode_coproc_m2il, arm_decode_data_i2il, arm_decode_data_misc2il, arm_decode_data_processing2il, arm_decode_data_r2il, arm_decode_data_rd02il, arm_decode_data_rn02il, arm_decode_data_rsr2il, arm_decode_extend2il, arm_decode_extra_load_store2il, arm_decode_extra_ls_i2il, arm_decode_extra_ls_r2il, arm_decode_floating_data_processing2il, arm_decode_halfword_multiply2il, arm_decode_hint2il, arm_decode_hmul2il, arm_decode_load_store2il, arm_decode_ls_i2il,
+arm_decode_lsm2il, arm_decode_ls_r2il, arm_decode_media2il, arm_decode_mem_hint_simd2il, arm_decode_misc2il, arm_decode_mov_wt2il, arm_decode_msr_hints2il,
+arm_decode_mul2il, arm_decode_multiply2il, arm_decode_packing2il, arm_decode_parallel_add_sub2il, arm_decode_pas2il, arm_decode_pld_i2il, arm_decode_pld_r2il, arm_decode_rev2il, arm_decode_sat2il, arm_decode_saturating_add_sub2il,
+arm_decode_signed_multiply2il, arm_decode_simd2il, arm_decode_svc2il, arm_decode_sync_l2il, arm_decode_sync_primitives2il, arm_decode_sync_s2il, arm_decode_unconditional2il, arm_decode_vcmp2il, arm_decode_vcvt_ds2il, arm_decode_vcvt_fpf2il, arm_decode_vcvt_fpi2il, arm_decode_vfp2il,
+arm_decode_vfp_other2il, arm_decode_vls2il, arm_decode_vlsm2il, arm_decode_vmov_i2il, arm_decode_vmov_r12il, arm_decode_vmov_r22il, arm_decode_vmrs2il, arm_decode_vreg_ls2il,
+arm_decode_vls2il, arm_decode_64bit_transfer2il, arm_decode_8_16_32bit_transfer2il, arm_decode_b2il, arm_decode_bfx2il, arm_decode_bkpt2il, arm_decode_bl2il, arm_decode_blx_i2il, arm_decode_blx_r2il, arm_decode_bx2il, arm_decode_bxj2il, arm_decode_clz2il, arm_decode_data_i2il, arm_decode_extend2il, arm_decode_hint2il, arm_decode_mem_hint_simd2il, arm_decode_mul2il, arm_decode_sat2il, arm_decode_sync_l2il, arm_decode_vlsm2il,
+arm_decode_pld_i2il, arm_decode_pld_r2il, arm_decode_simd2il, arm_decode_vmov_r12il, arm_decode_vmov_r22il, arm_decode_vmrs2il.
+unfold arm2il.
+Print Z.of_N.
+Abort.
+
+(* Example of zxbits we want to convert to xbits and N
+ else
+  if (zxbits (Z.of_N x) Z28 Z32 =? Z15)%Z
+  then
+   if
+    (zxbits (zxbits (Z.of_N x) Z20 Z28) Z5 Z8 =? 0)%Z
+    || (zxbits (zxbits (Z.of_N x) Z20 Z28) Z5 Z8 =? Z1)%Z
+    || (zxbits (zxbits (Z.of_N x) Z20 Z28) Z5 Z8 =? Z2)%Z
+    || (zxbits (zxbits (Z.of_N x) Z20 Z28) Z5 Z8 =? Z3)%Z
+   then
+    if (zxbits (zxbits (Z.of_N x) Z20 Z27) Z4 Z7 =? 0)%Z
+    then Move R_PC (Word (a mod 2 ^ 32) 32) $; Exn 4
+    else
+     if (zxbits (zxbits (Z.of_N x) Z20 Z27) Z4 Z7 =? Z1)%Z
+ *)
+
+Print term.
+
+Require Import ZArith.
+
+Locate Z_xbits_nonneg.
+
+  Search Z_xbits.
+  Search Z.to_N 0%Z.
+Compute arm2il a (arm_decode (Z.of_N x)).
+Check arm_prog : store -> addr -> option (N * stmt) .
+Print arm_prog.
+Print TemplateMonad.
+Print term.
+
+Definition printDef (q : qualid): TemplateMonad unit :=
+  gref <- tmLocate1 q ;;
+  match gref with
+  | IndRef ind => mib <- (tmQuoteInductive ind.(inductive_mind));; tmPrint mib
+  | ConstRef kn => cstb <- (tmQuoteConstant kn false);; tmPrint cstb
+  | _ => tmFail ("[" ++ q ++ "] is not an inductive")
+  end.
+
+Print constant_body.
+MetaRocq Run (printDef "xbits").
+
+Compute $quote 1%N.
+                     [tApp
+                        (tConstruct
+                           {|
+                             inductive_mind :=
+                               (MPfile ["BinNums"; "Numbers"; "Corelib"], "N");
+                             inductive_ind := 0
+                           |} 1 [])
+                        [tApp
+                           (tConstruct
+                              {|
+                                inductive_mind :=
+                                  (MPfile ["BinNums"; "Numbers"; "Corelib"],
+                                   "positive");
+                                inductive_ind := 0
+                              |} 1 [])
+                           [tConstruct
+                              {|
+                                inductive_mind :=
+                                  (MPfile ["BinNums"; "Numbers"; "Corelib"],
+                                   "positive");
+                                inductive_ind := 0
+                              |} 2 []]];
+Compute printDef "xbits".
+
+Definition printInductive (q : qualid): TemplateMonad unit :=
+  kn <- tmLocate1 q ;;
+  match kn with
+  | IndRef ind => mib <- (tmQuoteInductive ind.(inductive_mind));; tmPrint mib
+  | _ => tmFail ("[" ++ q ++ "] is not an inductive")
+  end.
+
+Compute ($quote arm_prog).
+MetaRocq Test Quote arm_prog.
+Search arm2il.
