Picinae_pilbox64.v
@@ -1,6 +1,6 @@
 (* Picinae: Platform In Coq for INstruction Analysis of Executables       ZZM7DZ
                                                                           $MNDM7
-   Copyright (c) 2025 Kevin W. Hamlen            ,,A??=P                 OMMNMZ+
+   Copyright (c) 2023 Kevin W. Hamlen            ,,A??=P                 OMMNMZ+
    The University of Texas at Dallas         =:$ZZ$+ZZI                  7MMZMZ7
    Computer Science Department             Z$$ZM++O++                    7MMZZN+
                                           ZZ$7Z.ZM~?                     7MZDNO$
@@ -11,7 +11,7 @@
                                                      MMM8MMMMMMMMMMM77   +MMMMZZ
                                                      MMMMMMMMMMMZMDMD77$.ZMZMM78
                                                       MMMMMMMMMMMMMMMMMMMZOMMM+Z
-   Instantiation of Picinae for ARMv7 ISA.             MMMMMMMMMMMMMMMMM^NZMMN+Z
+   Instantiation of Picinae for PILbox64 ISA.          MMMMMMMMMMMMMMMMM^NZMMN+Z
                                                         MMMMMMMMMMMMMMM/.$MZM8O+
    To compile this module, first load and compile:       MMMMMMMMMMMMMM7..$MNDM+
    * Picinae_core                                         MMDMMMMMMMMMZ7..$DM$77
@@ -38,57 +38,34 @@ Require Export Picinae_statics.
 Require Export Picinae_finterp.
 Require Export Picinae_simplifier_v1_1.
 Require Export Picinae_ISA.
+Require Export Picinae_auto.
 Require Import NArith.
 Require Import Program.Equality.
 Require Import Structures.Equalities.
 Open Scope N.
 
 (* Variables found in IL code lifted from ARM native code: *)
-Inductive arm7var :=
-  (* Main memory: support both 32 bit(ARMv1-v8) mode and 64 bit(ARMv8) *)
-  | V_MEM32 | V_MEM64
-  (* Floating point (VFP) support and SIMD (NEON) are optional extensions to the ARMv7-A profile.*)
-  (* ARM’s pc register is analogous to IA-32’s EIP register *)
-  | R_R0 | R_R1 | R_R2 | R_R3 | R_R4 | R_R5 | R_R6 | R_R7
-  | R_R8 | R_R9 | R_R10 | R_R11 | R_R12
-  (* R13: stack pointer | R14: link register | R15: program counter *)
-  | R_SP | R_LR | R_PC
-  (* Current Program Status Register (CPSR)*)
-  | R_M (* (bits 0–4) are the processor mode bits.*)
-  | R_T (* (bit 5) is the Thumb state bit. *)
-  | R_F (* (bit 6) is the FIQ disable bit. *)
-  | R_I (* (bit 7) is the IRQ disable bit. *)
-  | R_A (* (bit 8) is the imprecise data abort disable bit. *)
-  | R_E (* (bit 9) is the data endianness bit. *)
-  | R_IT (* (bits 10–15 and 25–26) is the if-then state bits. *)
-  | R_GE (* (bits 16–19) is the greater-than-or-equal-to bits. *)
-  | R_DNM (* (bits 20–23) is the do not modify bits. *)
-  | R_JF (* (bit 24) is the Java state bit. *)
-  | R_QF (* (bit 27) is the sticky overflow bit. *)
-  | R_VF (* (bit 28) is the overflow bit. *)
-  | R_CF (* (bit 29) is the carry/borrow/extend bit. *)
-  | R_ZF (* (bit 30) is the zero bit. *)
-  | R_NF (* (bit 31) is the negative/less than bit. *)
+Inductive pil64var :=
+  (* Main memory: 64 bit-width addresses, 2^64 bytes *)
+  | V_MEM64
+  (* 0-5, SP, LR = 64bit registers. *)
+  | R_R0 | R_R1 | R_R2 | R_R3 | R_R4 | R_R5
+  (* SP = stack pointer *)
+  | R_SP
+  (* LR = link register *)
+  | R_LR
+  (* PC = program counter *)
+  | R_PC
   (* These meta-variables model page access permissions: *)
-  | A_READ | A_WRITE
-  | V_TEMP (n:N) (* Temporaries introduced by the lifter: *).
+  | A_READ | A_WRITE | A_EXEC.
 
 (* Declare the types (i.e., bitwidths) of all the CPU registers: *)
-Definition arm7typctx v :=
-  match v with
-  | V_MEM32 => Some (8*2^32)
+Definition pil64typctx (id:pil64var) : option N :=
+  match id with
   | V_MEM64 => Some (8*2^64)
-  | R_R0 | R_R1 | R_R2 | R_R3 | R_R4 | R_R5 | R_R6 | R_R7 => Some 32
-  | R_R8 | R_R9 | R_R10 | R_R11 | R_R12 => Some 32
-  | R_SP | R_LR | R_PC => Some 32
-  | R_M => Some 5
-  | R_T | R_F | R_I | R_A | R_E => Some 1
-  | R_IT => Some 8
-  | R_GE => Some 4
-  | R_DNM => Some 4
-  | R_JF | R_QF | R_VF | R_CF | R_ZF | R_NF => Some 1
-  | A_READ | A_WRITE => Some (2^32)
-  | V_TEMP _ => None
+  | R_R0 | R_R1 | R_R2 | R_R3 | R_R4 | R_R5 => Some 64
+  | R_SP | R_LR | R_PC => Some 64
+  | A_READ | A_WRITE | A_EXEC => Some (2^64)
 end.
 
 (* Create a UsualDecidableType module (which is an instance of Typ) to give as
@@ -96,62 +73,73 @@ end.
    identifiers chosen above are syntactically written and how to decide whether
    any two variable instances refer to the same variable. *)
 
-Module MiniARM7VarEq <: MiniDecidableType.
-  Definition t := arm7var.
-  Definition eq_dec (v1 v2:arm7var) : {v1=v2}+{v1<>v2}.
+Module MiniPIL64VarEq <: MiniDecidableType.
+  Definition t := pil64var.
+  Definition eq_dec (v1 v2:pil64var) : {v1=v2}+{v1<>v2}.
     decide equality; apply N.eq_dec.
   Defined.  (* <-- This must be Defined (not Qed!) for finterp to work! *)
   Arguments eq_dec v1 v2 : simpl never.
-End MiniARM7VarEq.
+End MiniPIL64VarEq.
 
-Module ARM7Arch <: Architecture.
-  Module Var := Make_UDT MiniARM7VarEq.
+Module PIL64Arch <: Architecture.
+  Module Var := Make_UDT MiniPIL64VarEq.
   Definition var := Var.t.
   Definition store := var -> N.
   Definition typctx := var -> option bitwidth.
-  Definition archtyps := arm7typctx.
+  Definition archtyps := pil64typctx.
 
   Definition mem_readable s a := N.testbit (s A_READ) a = true.
   Definition mem_writable s a := N.testbit (s A_WRITE) a = true.
-End ARM7Arch.
+End PIL64Arch.
 
 (* Instantiate the Picinae modules with the arm identifiers above. *)
-Module IL_arm7 := PicinaeIL ARM7Arch.
-Export IL_arm7.
-Module Theory_arm7 := PicinaeTheory IL_arm7.
-Export Theory_arm7.
-Module Statics_arm7 := PicinaeStatics IL_arm7 Theory_arm7.
-Export Statics_arm7.
-Module FInterp_arm7 := PicinaeFInterp IL_arm7 Theory_arm7 Statics_arm7.
-Export FInterp_arm7.
-Module PSimpl_arm7 := Picinae_Simplifier_Base IL_arm7.
-Export PSimpl_arm7.
-Module PSimpl_arm7_v1_1 := Picinae_Simplifier_v1_1 IL_arm7 Theory_arm7 Statics_arm7 FInterp_arm7.
-Ltac PSimpl_arm7.PSimplifier ::= PSimpl_arm7_v1_1.PSimplifier.
+Module IL_pil64 := PicinaeIL PIL64Arch.
+Export IL_pil64.
+Module Theory_pil64 := PicinaeTheory IL_pil64.
+Export Theory_pil64.
+Module Statics_pil64 := PicinaeStatics IL_pil64 Theory_pil64.
+Export Statics_pil64.
+Module Auto_pil64 := PicinaeAuto IL_pil64 Theory_pil64 Statics_pil64.
+Export Auto_pil64.
+Module FInterp_pil64 := PicinaeFInterp IL_pil64 Theory_pil64 Statics_pil64.
+Export FInterp_pil64.
+Module PSimpl_pil64 := Picinae_Simplifier_Base IL_pil64.
+Export PSimpl_pil64.
+Module PSimpl_pil64_v1_1 := Picinae_Simplifier_v1_1 IL_pil64 Theory_pil64 Statics_pil64 FInterp_pil64.
+Ltac PSimpl_pil64.PSimplifier ::= PSimpl_pil64_v1_1.PSimplifier.
+
+Module ISA_pil64 := Picinae_ISA IL_pil64 PSimpl_pil64 Theory_pil64 Statics_pil64 FInterp_pil64.
+Export ISA_pil64.
+
+(* Introduce unique aliases for tactics in case user loads multiple architectures. *)
+Tactic Notation "pil64_psimpl" uconstr(e) "in" hyp(H) := psimpl_exp_hyp uconstr:(e) H.
+Tactic Notation "pil64_psimpl" uconstr(e) := psimpl_exp_goal uconstr:(e).
+Tactic Notation "pil64_psimpl" "in" hyp(H) := psimpl_hyp H.
+Tactic Notation "pil64_psimpl" := psimpl_goal.
+Ltac pil64_step := ISA_step.
 
 (* To use a different simplifier version (e.g., v1_0) put the following atop
    your proof .v file:
 Require Import Picinae_simplifier_v1_0.
-Module PSimpl_arm7_v1_0 := Picinae_Simplifier_v1_0 IL_arm7 Theory_arm7 Statics_arm7 FInterp_arm7.
-Ltac PSimpl_arm7.PSimplifier ::= PSimpl_arm7_v1_0.PSimplifier.
+Module PSimpl_pil64_v1_0 := Picinae_Simplifier_v1_0 IL_pil64 Statics_pil64 FInterp_pil64.
+Ltac PSimpl_pil64.PSimplifier ::= PSimpl_pil64_v1_0.PSimplifier.
 *)
 
-Module ISA_arm7 := Picinae_ISA IL_arm7 PSimpl_arm7 Theory_arm7 Statics_arm7 FInterp_arm7.
-Export ISA_arm7.
+(* Declare which context values are used to define store equivalence *)
+Definition pil64equivctx (id:var) : bool :=
+  match id with
+  | V_MEM64
+  | R_R0 | R_R1 | R_R2 | R_R3 | R_R4 | R_R5
+  | R_SP | R_LR => true
+  | _ => false
+  end.
+Definition pil64equiv (s1 s2:store) :=
+  forall (v:pil64var), pil64equivctx v = true -> s1 v = s2 v.
+Definition pil64equiv_or (s1 s2:store) (or_exception : pil64var -> bool) :=
+  forall (v:pil64var), pil64equivctx v = true -> or_exception v = true \/ s1 v = s2 v.
 
-(* Introduce unique aliases for tactics in case user loads multiple architectures. *)
-Tactic Notation "arm7_psimpl" uconstr(e) "in" hyp(H) := psimpl_exp_hyp uconstr:(e) H.
-Tactic Notation "arm7_psimpl" uconstr(e) := psimpl_exp_goal uconstr:(e).
-Tactic Notation "arm7_psimpl" "in" hyp(H) := psimpl_hyp H.
-Tactic Notation "arm7_psimpl" := psimpl_goal.
-Ltac arm7_step := ISA_step.
-
-(* The following is needed when applying cframe theorems from Picinae_theory. *)
-Theorem memacc_respects_arm7typctx: memacc_respects_typctx arm7typctx.
-Proof.
-  intros s1 s2 RV. rewrite <- RV. split; reflexivity.
-Qed.
-
+(* TODO: how should we change the memory access machinery?
+         How does it work anyhoo? *)
 (* Simplify memory access propositions by observing that on arm, the only part
    of the store that affects memory accessibility are the page-access bits
    (A_READ and A_WRITE). *)
@@ -188,6 +176,14 @@ Proof.
   intros. unfold MemAcc, mem_writable. rewrite !update_updated. reflexivity.
 Qed.
 
+Ltac simpl_memaccs H ::=
+  try lazymatch type of H with context [ MemAcc mem_writable ] =>
+    rewrite ?memacc_write_frame, ?memacc_write_updated in H by discriminate 1
+  end;
+  try lazymatch type of H with context [ MemAcc mem_readable ] =>
+    rewrite ?memacc_read_frame, ?memacc_read_updated in H by discriminate 1
+  end.
+
 (* Simplify arm memory access assertions produced by step_stmt. *)
 Ltac simpl_memaccs H ::=
   try lazymatch type of H with context [ MemAcc mem_writable ] =>
@@ -199,34 +195,28 @@ Ltac simpl_memaccs H ::=
 
 (* Define ISA-specific notations: *)
 
-Declare Scope arm7_scope.
-Delimit Scope arm7_scope with arm7.
-Bind Scope arm7_scope with stmt exp trace.
-Open Scope arm7_scope.
-Notation " s1 $; s2 " := (Seq s1 s2) (at level 75, right associativity) : arm7_scope.
+Declare Scope pil64_scope.
+Delimit Scope pil64_scope with pil64.
+Bind Scope pil64_scope with stmt exp trace.
+Open Scope pil64_scope.
+Notation " s1 $; s2 " := (Seq s1 s2) (at level 75, right associativity) : pil64_scope.
 
-Module ARM7Notations.
+Module PIL64Notations.
 
-Notation "m Ⓑ[ a  ]" := (getmem 32 LittleE 1 m a) (at level 30) : arm7_scope. (* read byte from memory *)
-Notation "m Ⓦ[ a  ]" := (getmem 32 LittleE 2 m a) (at level 30) : arm7_scope. (* read word from memory *)
-Notation "m Ⓓ[ a  ]" := (getmem 32 LittleE 4 m a) (at level 30) : arm7_scope. (* read dword from memory *)
-Notation "m Ⓠ[ a  ]" := (getmem 32 LittleE 8 m a) (at level 30) : arm7_scope. (* read quad word from memory *)
-Notation "m Ⓧ[ a  ]" := (getmem 32 LittleE 16 m a) (at level 30) : arm7_scope. (* read xmm from memory *)
-Notation "m Ⓨ[ a  ]" := (getmem 32 LittleE 32 m a) (at level 30) : arm7_scope. (* read ymm from memory *)
-Notation "m [Ⓑ a := v  ]" := (setmem 32 LittleE 1 m a v) (at level 50, left associativity) : arm7_scope. (* write byte to memory *)
-Notation "m [Ⓦ a := v  ]" := (setmem 32 LittleE 2 m a v) (at level 50, left associativity) : arm7_scope. (* write word to memory *)
-Notation "m [Ⓓ a := v  ]" := (setmem 32 LittleE 4 m a v) (at level 50, left associativity) : arm7_scope. (* write dword to memory *)
-Notation "m [Ⓠ a := v  ]" := (setmem 32 LittleE 8 m a v) (at level 50, left associativity) : arm7_scope. (* write quad word to memory *)
-Notation "m [Ⓧ a := v  ]" := (setmem 32 LittleE 16 m a v) (at level 50, left associativity) : arm7_scope. (* write xmm to memory *)
-Notation "m [Ⓨ a := v  ]" := (setmem 32 LittleE 32 m a v) (at level 50, left associativity) : arm7_scope. (* write ymm to memory *)
-Notation "x ⊕ y" := ((x+y) mod 2^32) (at level 50, left associativity). (* modular addition *)
-Notation "x ⊖ y" := (msub 32 x y) (at level 50, left associativity). (* modular subtraction *)
-Notation "x ⊗ y" := ((x*y) mod 2^32) (at level 40, left associativity). (* modular multiplication *)
+Notation "m Ⓑ[ a  ]" := (getmem 64 LittleE 1 m a) (at level 30) : pil64_scope. (* read byte from memory *)
+Notation "m Ⓦ[ a  ]" := (getmem 64 LittleE 2 m a) (at level 30) : pil64_scope. (* read word from memory *)
+Notation "m Ⓓ[ a  ]" := (getmem 64 LittleE 4 m a) (at level 30) : pil64_scope. (* read dword from memory *)
+Notation "m [Ⓑ  a := v  ]" := (setmem 64 LittleE 1 m a v) (at level 50, left associativity) : pil64_scope. (* write byte to memory *)
+Notation "m [Ⓦ  a := v  ]" := (setmem 64 LittleE 2 m a v) (at level 50, left associativity) : pil64_scope. (* write word to memory *)
+Notation "m [Ⓓ  a := v  ]" := (setmem 64 LittleE 4 m a v) (at level 50, left associativity) : pil64_scope. (* write dword to memory *)
+Notation "x ⊕ y" := ((x+y) mod 2^64) (at level 50, left associativity). (* modular addition *)
+Notation "x ⊖ y" := (msub 64 x y) (at level 50, left associativity). (* modular subtraction *)
+Notation "x ⊗ y" := ((x*y) mod 2^64) (at level 40, left associativity). (* modular multiplication *)
 Notation "x << y" := (N.shiftl x y) (at level 55, left associativity). (* logical shift-left *)
 Notation "x >> y" := (N.shiftr x y) (at level 55, left associativity). (* logical shift-right *)
-Notation "x >>> y" := (ashiftr 32 x y) (at level 55, left associativity). (* arithmetic shift-right *)
+Notation "x >>> y" := (ashiftr 64 x y) (at level 55, left associativity). (* arithmetic shift-right *)
 Notation "x .& y" := (N.land x y) (at level 56, left associativity). (* logical and *)
 Notation "x .^ y" := (N.lxor x y) (at level 57, left associativity). (* logical xor *)
 Notation "x .| y" := (N.lor x y) (at level 58, left associativity). (* logical or *)
 
-End ARM7Notations.
+End PIL64Notations.
